proof: Quick cleanup/organization

examples/dynamic_isolation/Proof.v
@@ -35,7 +35,9 @@ Declare Scope log_scope.
 Delimit Scope log_scope with log.
 Infix "++" := log_app (right associativity, at level 60) : log_scope.
 
-
+(* TODO: Temporary *)
+Axiom __magic__ : forall T, T.
+Tactic Notation "__magic" := apply __magic__.
 
 Hint Rewrite @getenv_create : log_helpers.
 
@@ -51,36 +53,6 @@ Module TradPf (External: External_sig) (EnclaveParams: EnclaveParameters)
   Module TODO_SM := SecurityMonitor External EnclaveParams Params0 Params1.
 
   Import Interfaces.Common.
-
-(* TODO_MOVE *)
-Ltac destruct_one_var_with t :=
-  match goal with
-  | [ H: ?T |- _ ] => is_var H; destruct H; try t
-  end.
-Ltac destruct_vars_with t :=
-  repeat (destruct_one_var_with t).
-
-Ltac solve' :=
-  match goal with
-  | |- ?x = (fst ?x, snd ?x) =>
-    destruct x; reflexivity
-  | [ H: False |- _ ] => solve [ destruct H ]
-  | [ H: ?P |- ?P ] => exact H
-  end.
-
-Ltac rewrite_in_goal :=
-  repeat lazymatch goal with
-  | H: ?x = ?x |- _ =>  fail 1
-  | H: ?x = _ |- context[?x] =>
-      rewrite H
-  end.
-
-Ltac simplify_tupless := simplify_tuples; subst.
-
-
-Tactic Notation "destruct_one_var" := destruct_one_var_with auto.
-Tactic Notation "destruct_vars_with" tactic(t) := repeat (destruct_one_var_with t).
-Tactic Notation "destruct_vars" := destruct_vars_with auto.
 
   Section TODO_WF_Properties.
     Property wf_r_lift_core0:
@@ -323,6 +295,10 @@ Tactic Notation "destruct_vars" := destruct_vars_with auto.
                                 Core0.rules
                                 Core0.schedule.
 
+      Definition core0_valid_input := @Core_Common.valid_input Core0.private_params.
+      Definition core0_valid_output := @Core_Common.valid_output Params0.core_id Params0.initial_pc Core0.private_params External.ext Core0.rule_name_t Core0.rules Core0.schedule.
+      Definition core0_valid_feedback := @Core_Common.valid_feedback Params0.core_id Params0.initial_pc Core0.private_params External.ext Core0.rule_name_t Core0.rules Core0.schedule.
+      Definition core0_output_log_equivalent := @Core_Common.output_log_equivalent Core0.private_params.
 
 
 
@@ -388,7 +364,20 @@ Tactic Notation "destruct_vars" := destruct_vars_with auto.
                                 Core1.rules
                                 Core1.schedule.
 
+      Definition core1_output_log_equivalent := @Core_Common.output_log_equivalent Core1.private_params.
+      Definition core1_valid_input := @Core_Common.valid_input Core1.private_params.
+      Definition core1_valid_output := @Core_Common.valid_output Params1.core_id Params1.initial_pc Core1.private_params External.ext Core1.rule_name_t Core1.rules Core1.schedule.
+      Definition core1_valid_feedback := @Core_Common.valid_feedback Params1.core_id Params1.initial_pc Core1.private_params External.ext Core1.rule_name_t Core1.rules Core1.schedule.
+
+
   End Derived_Core1.
+
+  (* TODO: Get rid of this after finishing definitions *)
+  Section DerivedSm.
+      Definition sm_valid_input := @SM_Common.valid_input Params0.initial_pc Params1.initial_pc
+                                                          EnclaveParams.params External.ext.
+
+  End DerivedSm.
 
   Section Derived_Mem.
     Check Mem_Common.initial_spec_state.
@@ -460,6 +449,19 @@ Tactic Notation "destruct_vars" := destruct_vars_with auto.
                                Memory.private_external_state_t
                                Memory.initial_private_external_state
                                Memory.external_update_function.
+
+      (* TODO: fewer params after defining *)
+      Definition mem_valid_input := @Mem_Common.valid_input
+                                          Memory.private_params External.ext
+                                          EnclaveParams.params Memory.rule_name_t
+                                          Memory.rules Memory.schedule
+                                          Memory.private_external_state_t
+                                          Memory.initial_private_external_state
+                                          Memory.external_update_function.
+
+      Definition mem_output_log_equivalent :=
+        @Mem_Common.output_log_equivalent Memory.private_params.
+
 
   End Derived_Mem.
 
@@ -947,6 +949,227 @@ Tactic Notation "destruct_vars" := destruct_vars_with auto.
 
     End HelperLemmas.
 
+    Section ExtractStep.
+
+      Definition core0_input (impl_io: mod_step_io) : Core_Common.input_t :=
+        Core_Common.step_input (step_io_core0 impl_io).
+      Definition core1_input (impl_io: mod_step_io) : Core_Common.input_t :=
+        Core_Common.step_input (step_io_core1 impl_io).
+      Definition sm_input (impl_io: mod_step_io) : SM_Common.input_t :=
+        SM_Common.step_input (step_io_sm impl_io).
+      Definition mem_input (impl_io: mod_step_io) : Log Mem_Common.R_public ContextEnv  :=
+        Mem_Common.step_input (step_io_mem impl_io).
+      Definition core0_feedback (impl_io: mod_step_io) : Core_Common.feedback_t :=
+        Core_Common.step_feedback (step_io_core0 impl_io).
+      Definition core1_feedback (impl_io: mod_step_io) : Core_Common.feedback_t :=
+        Core_Common.step_feedback (step_io_core1 impl_io).
+      Definition sm_feedback (impl_io: mod_step_io) : SM_Common.feedback_t :=
+        SM_Common.step_feedback (step_io_sm impl_io).
+      Definition mem_feedback (impl_io: mod_step_io) : Log Mem_Common.R_public ContextEnv  :=
+        Mem_Common.step_feedback (step_io_mem impl_io).
+
+      Ltac extract_impl_step__start :=
+        intros; consider do_step_with_metadata; consider compute_mod_outputs;
+          fast_destruct_nongoal_matches; simplify_tupless; simpl in *.
+      (* slower QED *)
+      Ltac extract_impl_step__step :=
+        consider do_core0; fast_destruct_nongoal_matches; simplify_tupless; simpl in *;
+        consider do_core1; fast_destruct_nongoal_matches; simplify_tupless; simpl in *;
+        consider do_sm; fast_destruct_nongoal_matches; simplify_tupless; simpl in *;
+        consider do_mem; fast_destruct_nongoal_matches; simplify_tupless; simpl in *.
+
+      Hint Rewrite @SemanticProperties.log_app_empty_l : log_helpers.
+
+      (* NOTE: Easy to automate, but naive way makes the QED a tad slower? How do we do better? *)
+
+      Lemma do_step_core0_input_empty :
+        forall impl_st impl_st' impl_ev impl_io,
+        do_step_with_metadata impl_st = (impl_st', impl_ev, impl_io) ->
+        core0_input impl_io = log_empty.
+      Proof.
+        extract_impl_step__start.
+        extract_impl_step__step.
+        consider do_core0; fast_destruct_nongoal_matches; simplify_tupless; simpl in *.
+        consider @Core_Common.proj_log__pub.
+        apply_equiv_eq.
+        consider core0_input.
+        intros; autorewrite with log_helpers; auto.
+      Qed.
+
+      Lemma core0_do_step_output :
+        forall impl_st impl_st' impl_ev impl_io,
+        do_step_with_metadata impl_st = (impl_st', impl_ev, impl_io) ->
+        fst (core0_do_step_input__koika (state_core0 impl_st)
+                                      (core0_input impl_io)) =
+        output_core0 impl_ev.
+      Proof.
+        extract_impl_step__start.
+        consider do_core0; fast_destruct_nongoal_matches; simplify_tupless; simpl.
+        unfold_core0_steps.
+        autorewrite with log_helpers in *.
+        consider @Core_Common.do_step_input__koika; simplify_tupless.
+        auto.
+      Qed.
+
+      Lemma core0_do_step_feedback :
+        forall impl_st impl_st' impl_ev impl_io,
+        do_step_with_metadata impl_st = (impl_st', impl_ev, impl_io) ->
+        Core_Common.step_feedback (step_io_core0 impl_io) =
+        Core_Common.proj_log__pub
+          (proj_log (REnv' := ContextEnv) Impl.System.Lift_core0
+                    ((lift_log Impl.System.Lift_mem (output_mem impl_ev))++
+                     (lift_log Impl.System.Lift_sm (output_sm impl_ev))++
+                     (lift_log Impl.System.Lift_core1 (output_core1 impl_ev)))%log).
+      Proof.
+        extract_impl_step__start.
+        consider do_core0; fast_destruct_nongoal_matches; simplify_tupless; simpl.
+        consider do_core1; fast_destruct_nongoal_matches; simplify_tupless; simpl.
+        consider do_sm; fast_destruct_nongoal_matches; simplify_tupless; simpl.
+        consider do_mem; fast_destruct_nongoal_matches; simplify_tupless; simpl.
+        rewrite SemanticProperties.log_app_empty_r.
+        rewrite SemanticProperties.log_app_assoc; auto.
+      Qed.
+
+      Lemma core1_do_step_input :
+        forall impl_st impl_st' impl_ev impl_io,
+        do_step_with_metadata impl_st = (impl_st', impl_ev, impl_io) ->
+        core1_input impl_io =
+          Core_Common.proj_log__pub
+            (proj_log (REnv' := ContextEnv) Impl.System.Lift_core1 (lift_log Impl.System.Lift_core0 (output_core0 impl_ev))).
+      Proof.
+        extract_impl_step__start.
+        consider core1_input; simpl.
+        consider do_core1; fast_destruct_nongoal_matches; simplify_tupless; simpl.
+        consider do_core0; destruct_all_matches; simplify_tupless.
+        autorewrite with log_helpers; auto.
+      Qed.
+
+      Lemma core1_do_step_output :
+        forall impl_st impl_st' impl_ev impl_io,
+        do_step_with_metadata impl_st = (impl_st', impl_ev, impl_io) ->
+        fst (core1_do_step_input__koika (state_core1 impl_st)
+                                      (core1_input impl_io)) =
+        output_core1 impl_ev.
+      Proof.
+        extract_impl_step__start.
+        consider do_core1; fast_destruct_nongoal_matches; simplify_tupless; simpl.
+        unfold_core1_steps.
+        autorewrite with log_helpers in *.
+        consider @Core_Common.do_step_input__koika; simplify_tupless.
+        auto.
+      Qed.
+
+      Lemma core1_do_step_feedback :
+        forall impl_st impl_st' impl_ev impl_io,
+        do_step_with_metadata impl_st = (impl_st', impl_ev, impl_io) ->
+        Core_Common.step_feedback (step_io_core1 impl_io) =
+        Core_Common.proj_log__pub
+          (proj_log (REnv' := ContextEnv) Impl.System.Lift_core1
+                    ((lift_log Impl.System.Lift_mem (output_mem impl_ev))++
+                     (lift_log Impl.System.Lift_sm (output_sm impl_ev)))%log).
+      Proof.
+        extract_impl_step__start.
+        consider do_core1; fast_destruct_nongoal_matches; simplify_tupless; simpl.
+        consider do_sm; fast_destruct_nongoal_matches; simplify_tupless; simpl.
+        consider do_mem; fast_destruct_nongoal_matches; simplify_tupless; simpl.
+        rewrite SemanticProperties.log_app_empty_r; auto.
+      Qed.
+
+
+      Lemma sm_do_step_input :
+        forall impl_st impl_st' impl_ev impl_io,
+        do_step_with_metadata impl_st = (impl_st', impl_ev, impl_io) ->
+        sm_input impl_io =
+          SM_Common.proj_log__pub
+            (proj_log (REnv' := ContextEnv) Impl.System.Lift_sm
+                      ((lift_log Impl.System.Lift_core1 (output_core1 impl_ev)) ++ (lift_log Impl.System.Lift_core0 (output_core0 impl_ev)))%log).
+      Proof.
+        extract_impl_step__start.
+        consider do_sm; fast_destruct_nongoal_matches; simplify_tupless; simpl.
+        consider do_core1; fast_destruct_nongoal_matches; simplify_tupless; simpl.
+        consider do_core0; destruct_all_matches; simplify_tupless.
+        autorewrite with log_helpers; auto.
+      Qed.
+
+
+      Lemma sm_do_step_output :
+        forall impl_st impl_st' impl_ev impl_io,
+        do_step_with_metadata impl_st = (impl_st', impl_ev, impl_io) ->
+        fst (Impl.System.SM.do_step_input__impl (state_sm impl_st)
+                                              (sm_input impl_io)) =
+        output_sm impl_ev.
+      Proof.
+        extract_impl_step__start.
+        consider do_sm; fast_destruct_nongoal_matches; simplify_tupless; simpl.
+        unfold_sm_steps.
+        autorewrite with log_helpers in *.
+        consider @SM_Common.do_step_input__impl; simplify_tupless.
+        auto.
+      Qed.
+
+      Lemma sm_do_step_feedback :
+        forall impl_st impl_st' impl_ev impl_io,
+        do_step_with_metadata impl_st = (impl_st', impl_ev, impl_io) ->
+        SM_Common.step_feedback (step_io_sm impl_io) =
+        SM_Common.proj_log__pub
+          (proj_log (REnv' := ContextEnv) Impl.System.Lift_sm
+                    (lift_log Impl.System.Lift_mem (output_mem impl_ev))).
+      Proof.
+        extract_impl_step__start.
+        consider do_sm; fast_destruct_nongoal_matches; simplify_tupless; simpl.
+        consider do_mem; fast_destruct_nongoal_matches; simplify_tupless; simpl.
+        rewrite SemanticProperties.log_app_empty_r; auto.
+      Qed.
+
+
+
+
+      Lemma mem_do_step_input :
+        forall impl_st impl_st' impl_ev impl_io,
+        do_step_with_metadata impl_st = (impl_st', impl_ev, impl_io) ->
+        mem_input impl_io =
+          Mem_Common.proj_log__pub
+            (proj_log (REnv' := ContextEnv) Impl.System.Lift_mem
+                      ((lift_log Impl.System.Lift_sm (output_sm impl_ev)) ++
+                       (lift_log Impl.System.Lift_core1 (output_core1 impl_ev)) ++
+                       (lift_log Impl.System.Lift_core0 (output_core0 impl_ev)))%log).
+      Proof.
+        extract_impl_step__start.
+        consider mem_input; simpl.
+        consider do_mem; fast_destruct_nongoal_matches; simplify_tupless; simpl.
+        consider do_sm; fast_destruct_nongoal_matches; simplify_tupless; simpl.
+        consider do_core1; fast_destruct_nongoal_matches; simplify_tupless; simpl.
+        consider do_core0; destruct_all_matches; simplify_tupless.
+        autorewrite with log_helpers; auto.
+      Qed.
+
+      Lemma mem_do_step_output :
+        forall impl_st impl_st' impl_ev impl_io,
+        do_step_with_metadata impl_st = (impl_st', impl_ev, impl_io) ->
+        fst (mem_do_step_input__impl (state_mem impl_st)
+                                   (mem_input impl_io)) =
+        output_mem impl_ev.
+      Proof.
+        extract_impl_step__start.
+        consider mem_input.
+        consider do_mem; fast_destruct_nongoal_matches; simplify_tupless; simpl.
+        autorewrite with log_helpers in *.
+        rewrite_solve.
+      Qed.
+
+      Lemma do_step_mem_feedback_empty :
+        forall impl_st impl_st' impl_ev impl_io,
+        do_step_with_metadata impl_st = (impl_st', impl_ev, impl_io) ->
+        mem_feedback impl_io = log_empty.
+      Proof.
+        extract_impl_step__start.
+        consider do_mem; fast_destruct_nongoal_matches; simplify_tupless; simpl in *.
+        apply_equiv_eq.
+        consider mem_feedback; simpl.
+        intros; autorewrite with log_helpers; auto.
+      Qed.
+    End ExtractStep.
+
   End ModImpl.
 
   Module ModSpec.
@@ -1411,6 +1634,234 @@ Tactic Notation "destruct_vars" := destruct_vars_with auto.
 
     End HelperLemmas.
 
+    Section ExtractStep.
+      Definition core0_input (spec_io: mod_step_io) : Core_Common.input_t :=
+        Core_Common.step_input (step_io_core0 spec_io).
+      Definition core1_input (spec_io: mod_step_io) : Core_Common.input_t :=
+        Core_Common.step_input (step_io_core1 spec_io).
+      Definition sm_input (spec_io: mod_step_io) : SM_Common.input_t :=
+        SM_Common.step_input (fst (step_io_sm spec_io)).
+      Definition mem_input (spec_io: mod_step_io) : Mem_Common.input_t :=
+        (Mem_Common.step_input (Mem_Common.ghost_step (step_io_mem spec_io)),
+         (Mem_Common.ghost_input_config0 (step_io_mem spec_io),
+          Mem_Common.ghost_input_config1 (step_io_mem spec_io))).
+      Definition core0_feedback (spec_io: mod_step_io) : Core_Common.feedback_t :=
+        Core_Common.step_feedback (step_io_core0 spec_io).
+      Definition core1_feedback (spec_io: mod_step_io) : Core_Common.feedback_t :=
+        Core_Common.step_feedback (step_io_core1 spec_io).
+      Definition sm_feedback (spec_io: mod_step_io) : SM_Common.feedback_t :=
+        SM_Common.step_feedback (fst (step_io_sm spec_io)).
+      Definition mem_feedback (spec_io: mod_step_io) : Mem_Common.feedback_t :=
+        (Mem_Common.step_feedback (Mem_Common.ghost_step (step_io_mem spec_io))).
+
+      Ltac extract_spec_step__start :=
+        intros; consider do_step_with_metadata; consider compute_mod_outputs;
+          fast_destruct_nongoal_matches; simplify_tupless; simpl in *.
+
+      Lemma do_step_core0_input_empty :
+        forall spec_st spec_st' spec_ev spec_io,
+        do_step_with_metadata spec_st = (spec_st', spec_ev, spec_io) ->
+        core0_input spec_io = log_empty.
+      Proof.
+        extract_spec_step__start.
+        consider do_core0; fast_destruct_nongoal_matches; simplify_tupless; simpl in *.
+        consider @Core_Common.proj_log__pub.
+        apply_equiv_eq.
+        intros; autorewrite with log_helpers; auto.
+      Qed.
+
+      Lemma core0_do_step_output :
+        forall spec_st spec_st' spec_ev spec_io,
+        do_step_with_metadata spec_st = (spec_st', spec_ev, spec_io) ->
+        fst (core0_do_step_trans_input__spec (state_core0 spec_st) (core0_input spec_io)) =
+        output_core0 spec_ev.
+      Proof.
+        extract_spec_step__start.
+        consider do_core0; fast_destruct_nongoal_matches; simplify_tupless.
+        unfold_core0_steps.
+        autorewrite with log_helpers in *.
+        consider @Core_Common.proj_log__pub.
+        consider @Core_Common.do_step_trans_input__spec; consider @Core_Common.do_step_input__koika; simplify_tupless.
+        simpl.
+        consider core0_input; simpl.
+        auto.
+      Qed.
+
+      Lemma core0_do_step_feedback :
+        forall spec_st spec_st' spec_ev spec_io,
+          do_step_with_metadata spec_st = (spec_st', spec_ev, spec_io) ->
+          Core_Common.step_feedback (step_io_core0 spec_io) =
+          Core_Common.proj_log__pub
+            (proj_log (REnv' := ContextEnv) Impl.System.Lift_core0
+                      ((lift_log Impl.System.Lift_mem (combine_mem_public_output ((output_mem spec_ev))))++
+                      (lift_log Impl.System.Lift_sm (fst (combine_sm_public_output (output_sm spec_ev))))++
+                      (lift_log Impl.System.Lift_core1 (output_core1 spec_ev)))%log).
+      Proof.
+        extract_spec_step__start.
+        rewrite SemanticProperties.log_app_empty_r; auto.
+        consider do_mem; fast_destruct_nongoal_matches; simplify_tupless; simpl.
+        consider do_sm; fast_destruct_nongoal_matches; simplify_tupless; simpl.
+        consider do_core1; fast_destruct_nongoal_matches; simplify_tupless; simpl.
+        consider do_core0; fast_destruct_nongoal_matches; simplify_tupless; simpl.
+        rewrite SemanticProperties.log_app_assoc; auto.
+        rewrite Heqp0; simpl.
+        repeat rewrite SemanticProperties.log_app_assoc; auto.
+      Qed.
+
+      Lemma core1_do_step_input :
+        forall spec_st spec_st' spec_ev spec_io,
+        do_step_with_metadata spec_st = (spec_st', spec_ev, spec_io) ->
+        core1_input spec_io =
+          Core_Common.proj_log__pub
+            (proj_log (REnv' := ContextEnv) Impl.System.Lift_core1 (lift_log Impl.System.Lift_core0 (output_core0 spec_ev))).
+      Proof.
+        extract_spec_step__start.
+        consider core1_input; simpl.
+        consider do_core1; fast_destruct_nongoal_matches; simplify_tupless; simpl.
+        consider do_core0; fast_destruct_nongoal_matches; simplify_tupless; simpl.
+        rewrite SemanticProperties.log_app_empty_l.
+        auto.
+      Qed.
+
+      Lemma core1_do_step_output :
+        forall spec_st spec_st' spec_ev spec_io,
+        do_step_with_metadata spec_st = (spec_st', spec_ev, spec_io) ->
+        fst (core1_do_step_trans_input__spec (state_core1 spec_st) (core1_input spec_io)) =
+        output_core1 spec_ev.
+      Proof.
+        extract_spec_step__start.
+        consider do_core1; fast_destruct_nongoal_matches; simplify_tupless.
+        unfold_core1_steps.
+        autorewrite with log_helpers in *.
+        consider @Core_Common.proj_log__pub.
+        consider @Core_Common.do_step_trans_input__spec; consider @Core_Common.do_step_input__koika; simplify_tupless.
+        simpl.
+        consider core1_input; simpl.
+        auto.
+      Qed.
+
+      Lemma core1_do_step_feedback :
+        forall spec_st spec_st' spec_ev spec_io,
+          do_step_with_metadata spec_st = (spec_st', spec_ev, spec_io) ->
+          Core_Common.step_feedback (step_io_core1 spec_io) =
+          Core_Common.proj_log__pub
+            (proj_log (REnv' := ContextEnv) Impl.System.Lift_core1
+                      ((lift_log Impl.System.Lift_mem (combine_mem_public_output ((output_mem spec_ev))))++
+                                                                                                                         (lift_log Impl.System.Lift_sm (fst (combine_sm_public_output (output_sm spec_ev))))%log)%log).
+      Proof.
+        extract_spec_step__start.
+        rewrite SemanticProperties.log_app_empty_r; auto.
+        consider do_mem; fast_destruct_nongoal_matches; simplify_tupless; simpl.
+        consider do_sm; fast_destruct_nongoal_matches; simplify_tupless; simpl.
+        consider do_core1; fast_destruct_nongoal_matches; simplify_tupless; simpl.
+        rewrite Heqp0; simpl.
+        rewrite SemanticProperties.log_app_assoc; auto.
+      Qed.
+
+      Lemma sm_do_step_input :
+        forall spec_st spec_st' spec_ev spec_io,
+        do_step_with_metadata spec_st = (spec_st', spec_ev, spec_io) ->
+        sm_input spec_io =
+          (SM_Common.proj_log__pub
+            (proj_log (REnv' := ContextEnv) Impl.System.Lift_sm
+                      ((lift_log Impl.System.Lift_core1 (output_core1 spec_ev)) ++
+                       (lift_log Impl.System.Lift_core0 (output_core0 spec_ev)))%log)).
+      Proof.
+        extract_spec_step__start.
+        consider sm_input; simpl.
+        consider do_sm; fast_destruct_nongoal_matches; simplify_tupless; simpl.
+        consider do_core1; fast_destruct_nongoal_matches; simplify_tupless; simpl.
+        consider do_core0; fast_destruct_nongoal_matches; simplify_tupless; simpl.
+        rewrite SemanticProperties.log_app_empty_l.
+        auto.
+      Qed.
+
+      Lemma sm_do_step_output :
+        forall spec_st spec_st' spec_ev spec_io,
+        do_step_with_metadata spec_st = (spec_st', spec_ev, spec_io) ->
+        Impl.System.SM.do_step_input__spec (state_sm spec_st)
+                                         (sm_input spec_io) =
+        output_sm spec_ev.
+      Proof.
+        extract_spec_step__start.
+        consider do_sm; fast_destruct_nongoal_matches; simplify_tupless.
+        unfold_sm_steps.
+        autorewrite with log_helpers in *; simpl.
+        consider sm_input; simpl.
+        auto.
+      Qed.
+
+      Lemma sm_do_step_feedback :
+        forall spec_st spec_st' spec_ev spec_io,
+          do_step_with_metadata spec_st = (spec_st', spec_ev, spec_io) ->
+          SM_Common.step_feedback (fst (step_io_sm spec_io)) =
+          SM_Common.proj_log__pub
+            (proj_log (REnv' := ContextEnv) Impl.System.Lift_sm
+                      (lift_log Impl.System.Lift_mem (combine_mem_public_output (output_mem spec_ev)))).
+      Proof.
+        extract_spec_step__start.
+        rewrite SemanticProperties.log_app_empty_r; auto.
+        consider do_mem; fast_destruct_nongoal_matches; simplify_tupless; simpl.
+        consider do_sm; fast_destruct_nongoal_matches; simplify_tupless; simpl.
+        auto.
+      Qed.
+
+      Lemma mem_do_step_input :
+        forall spec_st spec_st' spec_ev spec_io,
+        do_step_with_metadata spec_st = (spec_st', spec_ev, spec_io) ->
+        mem_input spec_io =
+          (Mem_Common.proj_log__pub
+            (proj_log (REnv' := ContextEnv) Impl.System.Lift_mem
+                      ((lift_log Impl.System.Lift_sm (fst (combine_sm_public_output (output_sm spec_ev)))) ++
+                       (lift_log Impl.System.Lift_core1 (output_core1 spec_ev)) ++
+                       (lift_log Impl.System.Lift_core0 (output_core0 spec_ev)))%log),
+            ((ghost_output_config0 (snd (combine_sm_public_output (output_sm spec_ev)))),
+             (ghost_output_config1 (snd (combine_sm_public_output (output_sm spec_ev)))))).
+      Proof.
+        extract_spec_step__start.
+        (* QED is faster with unfolding inputs? *)
+        consider mem_input; simpl.
+        consider sm_input; simpl.
+        consider core1_input; simpl.
+        consider core0_input; simpl.
+        consider do_mem; fast_destruct_nongoal_matches; simplify_tupless; simpl.
+        consider do_sm; fast_destruct_nongoal_matches; simplify_tupless; simpl.
+        consider do_core1; fast_destruct_nongoal_matches; simplify_tupless; simpl.
+        consider do_core0; fast_destruct_nongoal_matches; simplify_tupless; simpl.
+        rewrite Heqp0; simpl.
+        rewrite SemanticProperties.log_app_empty_l.
+        auto.
+      Qed.
+
+      Lemma mem_do_step_output :
+        forall spec_st spec_st' spec_ev spec_io,
+        do_step_with_metadata spec_st = (spec_st', spec_ev, spec_io) ->
+        mem_do_step_trans_input__spec (state_mem spec_st)
+                                    (mem_input spec_io) =
+        output_mem spec_ev.
+      Proof.
+        extract_spec_step__start.
+        consider do_mem; fast_destruct_nongoal_matches; simplify_tupless.
+        unfold_mem_steps.
+        autorewrite with log_helpers in *; simpl.
+        consider mem_input; simpl.
+        auto.
+      Qed.
+
+      Lemma do_step_mem_feedback_empty :
+        forall spec_st spec_st' spec_ev spec_io,
+        do_step_with_metadata spec_st = (spec_st', spec_ev, spec_io) ->
+        mem_feedback spec_io = log_empty.
+      Proof.
+        extract_spec_step__start.
+        consider do_mem; fast_destruct_nongoal_matches; simplify_tupless; simpl in *.
+        apply_equiv_eq.
+        consider mem_feedback; simpl.
+        intros; autorewrite with log_helpers; auto.
+      Qed.
+
+    End ExtractStep.
+
     Section Invariant.
       Definition InvariantState (st: state) : Prop. Admitted.
 
@@ -1469,6 +1920,30 @@ Tactic Notation "destruct_vars" := destruct_vars_with auto.
 
     End Invariant.
 
+    Section PropsLemmas.
+      Lemma valid_props_extract_core1_valid_input :
+        forall ios spec_st0 t initial_dram n,
+        step_n_with_metadata initial_dram n = (spec_st0, t, ios) ->
+        valid_props initial_dram (ios ++ [snd (do_step_with_metadata spec_st0)]) ->
+        core1_valid_input (state_core1 spec_st0) (core1_input (snd (do_step_with_metadata spec_st0))).
+      Admitted.
+
+      Lemma valid_props_extract_sm_valid_input :
+        forall ios spec_st0 t initial_dram n,
+        step_n_with_metadata initial_dram n = (spec_st0, t, ios) ->
+        valid_props initial_dram (ios ++ [snd (do_step_with_metadata spec_st0)]) ->
+        sm_valid_input (state_sm spec_st0) (sm_input (snd (do_step_with_metadata spec_st0))).
+      Admitted.
+
+      Lemma valid_props_extract_mem_valid_input :
+        forall ios spec_st0 t initial_dram n,
+        step_n_with_metadata initial_dram n = (spec_st0, t, ios) ->
+        valid_props initial_dram (ios ++ [snd (do_step_with_metadata spec_st0)]) ->
+        mem_valid_input (state_mem spec_st0) (mem_input (snd (do_step_with_metadata spec_st0))).
+      Admitted.
+
+    End PropsLemmas.
+
   End ModSpec.
 
   Module Observations.
@@ -1502,6 +1977,196 @@ Tactic Notation "destruct_vars" := destruct_vars_with auto.
   Module ModImplToModSpec.
     Import Observations.
     Import Interfaces.Common.
+
+    Section LiftProperties.
+
+      Ltac solve_lift_log_not_exists :=
+        repeat match goal with
+               | |- not (exists reg, rlift _ reg = _)  =>
+                 clear; intuition; simpl in *; destruct reg; simpl in *; try congruence
+               | H: Impl.System.mem_public_lift ?r = _ |- _ =>
+                 destruct r; simpl in *; try congruence
+               end.
+
+      Lemma cores_do_not_share_registers :
+        ~ (exists reg1 reg2, rlift Impl.System.Lift_core0 reg1 = rlift Impl.System.Lift_core1 reg2).
+      Proof.
+        intuition.
+        destruct reg1; destruct reg2; simpl in *;
+          consider Impl.System.Lift_core0; consider Impl.System.Lift_core1;
+            consider Impl.System.core0_public_lift; consider Impl.System.core1_public_lift;
+              destruct_all_matches; congruence.
+      Qed.
+
+      Lemma proj_core0_lift_core1_equiv :
+        forall log1 log2,
+          core1_output_log_equivalent log1 log2 ->
+          proj_log (REnv := ContextEnv) (REnv' := ContextEnv)
+                   Impl.System.Lift_core0 (lift_log Impl.System.Lift_core1 log1) =
+          proj_log (REnv' := ContextEnv) Impl.System.Lift_core0 (lift_log Impl.System.Lift_core1 log2).
+      Admitted.
+
+
+      Lemma proj_core0_lift_sm_equiv :
+        forall log1 log2,
+          SM_Common.output_log_equivalent log1 log2 ->
+          proj_log (REnv := ContextEnv) (REnv' := ContextEnv)
+                   Impl.System.Lift_core0 (lift_log Impl.System.Lift_sm log1) =
+          proj_log (REnv' := ContextEnv) Impl.System.Lift_core0 (lift_log Impl.System.Lift_sm (fst (ModSpec.combine_sm_public_output log2))).
+      Admitted.
+
+      Lemma proj_core0_lift_mem_equiv :
+        forall log1 log2,
+          mem_output_log_equivalent log1 log2 ->
+          proj_log (REnv := ContextEnv) (REnv' := ContextEnv)
+                   Impl.System.Lift_core0 (lift_log Impl.System.Lift_mem log1) =
+          proj_log (REnv' := ContextEnv) Impl.System.Lift_core0 (lift_log Impl.System.Lift_mem (ModSpec.combine_mem_public_output log2)).
+      Admitted.
+
+
+      Lemma proj_core1_lift_core0_log_equiv :
+        forall log1 log2,
+          Core_Common.proj_log__pub log1 = Core_Common.proj_log__pub log2 ->
+          proj_log (REnv := ContextEnv) (REnv' := ContextEnv)
+                   Impl.System.Lift_core1 (lift_log Impl.System.Lift_core0 log1) =
+          proj_log (REnv' := ContextEnv) Impl.System.Lift_core1 (lift_log Impl.System.Lift_core0 log2).
+      Proof.
+        intros.
+        consider @Core_Common.proj_log__pub.
+        consider @proj_log.
+        apply_equiv_eq.
+        intros.
+        repeat rewrite getenv_create.
+        destruct k.
+        - repeat rewrite getenv_lift_log_not_exists; auto;
+            intuition; apply cores_do_not_share_registers;
+              eexists; eexists; eauto.
+        - repeat rewrite getenv_lift_log_not_exists; auto;
+            intuition; apply cores_do_not_share_registers;
+              eexists; eexists; eauto.
+      Qed.
+
+      Lemma proj_core1_lift_sm_equiv :
+        forall log1 log2,
+          SM_Common.output_log_equivalent log1 log2 ->
+          proj_log (REnv := ContextEnv) (REnv' := ContextEnv)
+                   Impl.System.Lift_core1 (lift_log Impl.System.Lift_sm log1) =
+          proj_log (REnv' := ContextEnv) Impl.System.Lift_core1
+                   (lift_log Impl.System.Lift_sm (fst (ModSpec.combine_sm_public_output log2))).
+      Admitted.
+
+
+      Lemma proj_core1_lift_mem_equiv :
+        forall log1 log2,
+          mem_output_log_equivalent log1 log2 ->
+          proj_log (REnv := ContextEnv) (REnv' := ContextEnv)
+                   Impl.System.Lift_core1 (lift_log Impl.System.Lift_mem log1) =
+          proj_log (REnv' := ContextEnv) Impl.System.Lift_core1
+                   (lift_log Impl.System.Lift_mem (ModSpec.combine_mem_public_output log2)).
+      Admitted.
+
+      Lemma proj_sm_lift_core0_log_equiv :
+        forall log1 log1' ,
+          Core_Common.proj_log__pub log1 = Core_Common.proj_log__pub log1' ->
+          (proj_log (REnv := ContextEnv) (REnv' := ContextEnv) Impl.System.Lift_sm
+                    (lift_log Impl.System.Lift_core0 log1)) =
+          (proj_log (REnv' := ContextEnv) Impl.System.Lift_sm
+                    (lift_log Impl.System.Lift_core0 log1')).
+      Proof.
+        intros. consider @Core_Common.proj_log__pub.
+        consider @proj_log.
+        apply_equiv_eq; intros; repeat rewrite getenv_create.
+        destruct k.
+        - admit.
+        - repeat rewrite getenv_lift_log_not_exists; auto; intuition;
+            simpl in *; destruct reg; simpl in *; try congruence;
+              destruct r; simpl in *; congruence.
+      Admitted.
+
+      Lemma proj_sm_lift_core1_log_equiv :
+        forall log1 log1' ,
+          Core_Common.proj_log__pub log1 = Core_Common.proj_log__pub log1' ->
+          (proj_log (REnv := ContextEnv) (REnv' := ContextEnv) Impl.System.Lift_sm
+                    (lift_log Impl.System.Lift_core1 log1)) =
+          (proj_log (REnv' := ContextEnv) Impl.System.Lift_sm
+                    (lift_log Impl.System.Lift_core1 log1')).
+      Admitted.
+
+      Lemma sm_output_log_equiv_impl_combine_public_output :
+        forall impl_out spec_out,
+          SM_Common.output_log_equivalent impl_out spec_out ->
+          SM_Common.proj_log__pub impl_out =
+          SM_Common.proj_log__pub (fst (ModSpec.combine_sm_public_output spec_out)).
+      Proof.
+        intros. consider SM_Common.output_log_equivalent.
+        apply_equiv_eq.
+        intros. consider SM_Common.proj_log__pub.
+        repeat rewrite getenv_create.
+        consider ModSpec.combine_sm_public_output; simpl.
+        destruct spec_out; simpl. rewrite getenv_create.
+        specialize H with (reg := SM_Common.public k).
+        simpl in H.
+        destruct_all_matches; auto.
+      Qed.
+
+      Lemma proj_mem_lift_core0_log_equiv :
+        forall log1 log1' ,
+          Core_Common.proj_log__pub log1 = Core_Common.proj_log__pub log1' ->
+          (proj_log (REnv := ContextEnv) (REnv' := ContextEnv) Impl.System.Lift_mem
+                    (lift_log Impl.System.Lift_core0 log1)) =
+          (proj_log (REnv' := ContextEnv) Impl.System.Lift_mem
+                    (lift_log Impl.System.Lift_core0 log1')).
+      Admitted.
+
+      Lemma proj_mem_lift_core1_log_equiv :
+        forall log1 log1' ,
+          Core_Common.proj_log__pub log1 = Core_Common.proj_log__pub log1' ->
+          (proj_log (REnv := ContextEnv) (REnv' := ContextEnv) Impl.System.Lift_mem
+                    (lift_log Impl.System.Lift_core1 log1)) =
+          (proj_log (REnv' := ContextEnv) Impl.System.Lift_mem
+                    (lift_log Impl.System.Lift_core1 log1')).
+      Admitted.
+
+      Lemma proj_mem_lift_sm_log_equiv :
+        forall log1 log1' ,
+          SM_Common.proj_log__pub log1 = SM_Common.proj_log__pub log1' ->
+          (proj_log (REnv := ContextEnv) (REnv' := ContextEnv) Impl.System.Lift_mem
+                    (lift_log Impl.System.Lift_sm log1)) =
+          (proj_log (REnv' := ContextEnv) Impl.System.Lift_mem
+                    (lift_log Impl.System.Lift_sm log1')).
+      Admitted.
+
+      Lemma mem_output_log_equiv_impl_combine_public_output :
+        forall impl_out spec_out,
+          mem_output_log_equivalent impl_out spec_out ->
+          (proj_log (REnv := ContextEnv) (REnv' := ContextEnv)
+                    Impl.System.Lift_sm (lift_log Impl.System.Lift_mem impl_out)) =
+          (proj_log (REnv' := ContextEnv) Impl.System.Lift_sm
+                    (lift_log Impl.System.Lift_mem (ModSpec.combine_mem_public_output spec_out))).
+      Proof.
+        intros. consider mem_output_log_equivalent.
+        apply_equiv_eq.
+        intros; repeat rewrite getenv_create.
+        consider ModSpec.combine_mem_public_output; simpl.
+        destruct spec_out; simpl.
+        consider @Mem_Common.output_log_equivalent.
+        unfold proj_log. repeat rewrite getenv_create.
+        simpl_eqs.
+        destruct k; simpl.
+        - admit. (* lift annoying *)
+        - repeat rewrite getenv_lift_log_not_exists; auto;
+            solve_lift_log_not_exists.
+      Admitted.
+
+    End LiftProperties.
+
+    Ltac unfold_spec_props :=
+      consider ModSpec.valid_props;
+      consider ModSpec.valid_P_prop;
+      consider ModSpec.core0_P_prop;
+      consider ModSpec.core1_P_prop;
+      consider ModSpec.sm_P_prop;
+      consider ModSpec.mem_P_prop.
 
     Section Simulation.
 
@@ -1551,31 +2216,15 @@ Tactic Notation "destruct_vars" := destruct_vars_with auto.
         solve_forall_extract.
       Qed.
 
-      (* TODO: fewer params after defining *)
-      Definition core0_valid_input := @Core_Common.valid_input Core0.private_params.
-      Definition core0_valid_output := @Core_Common.valid_output Params0.core_id Params0.initial_pc Core0.private_params External.ext Core0.rule_name_t Core0.rules Core0.schedule.
-      Definition core0_valid_feedback := @Core_Common.valid_feedback Params0.core_id Params0.initial_pc Core0.private_params External.ext Core0.rule_name_t Core0.rules Core0.schedule.
-      Definition core0_output_log_equivalent := @Core_Common.output_log_equivalent Core0.private_params.
-      Definition core1_output_log_equivalent := @Core_Common.output_log_equivalent Core1.private_params.
-      Definition core1_valid_input := @Core_Common.valid_input Core1.private_params.
-      Definition core1_valid_output := @Core_Common.valid_output Params1.core_id Params1.initial_pc Core1.private_params External.ext Core1.rule_name_t Core1.rules Core1.schedule.
-      Definition core1_valid_feedback := @Core_Common.valid_feedback Params1.core_id Params1.initial_pc Core1.private_params External.ext Core1.rule_name_t Core1.rules Core1.schedule.
-
-      Definition sm_valid_input := @SM_Common.valid_input Params0.initial_pc Params1.initial_pc
-                                                          EnclaveParams.params External.ext.
-      Definition sm_output_log_equivalent :=
-        @SM_Common.output_log_equivalent.
-
-      Definition mem_valid_input := @Mem_Common.valid_input
-                                          Memory.private_params External.ext
-                                          EnclaveParams.params Memory.rule_name_t
-                                          Memory.rules Memory.schedule
-                                          Memory.private_external_state_t
-                                          Memory.initial_private_external_state
-                                          Memory.external_update_function.
-
-      Definition mem_output_log_equivalent :=
-        @Mem_Common.output_log_equivalent Memory.private_params.
+      Ltac unfold_short_ios :=
+        consider ModImpl.core0_input;
+        consider ModImpl.core1_input;
+        consider ModImpl.sm_input;
+        consider ModImpl.mem_input;
+        consider ModSpec.core0_input;
+        consider ModSpec.core1_input;
+        consider ModSpec.sm_input;
+        consider ModSpec.mem_input.
 
       Theorem step_n_ios_sim:
         forall initial_dram n impl_st impl_tr spec_st spec_tr impl_io spec_io,
@@ -1614,679 +2263,30 @@ Tactic Notation "destruct_vars" := destruct_vars_with auto.
           specialize ModSpec.step_n_invariant with (1 := HSpec); intros [HSpecInv HSpecProp]; propositional.
           propositional.
 
-
-Definition impl_core0_input (impl_io: ModImpl.mod_step_io) : Core_Common.input_t :=
-  Core_Common.step_input (ModImpl.step_io_core0 impl_io).
-Definition spec_core0_input (spec_io: ModSpec.mod_step_io) : Core_Common.input_t :=
-  Core_Common.step_input (ModSpec.step_io_core0 spec_io).
-Definition impl_core1_input (impl_io: ModImpl.mod_step_io) : Core_Common.input_t :=
-  Core_Common.step_input (ModImpl.step_io_core1 impl_io).
-Definition spec_core1_input (spec_io: ModSpec.mod_step_io) : Core_Common.input_t :=
-  Core_Common.step_input (ModSpec.step_io_core1 spec_io).
-Definition impl_sm_input (impl_io: ModImpl.mod_step_io) : SM_Common.input_t :=
-  SM_Common.step_input (ModImpl.step_io_sm impl_io).
-Definition spec_sm_input (spec_io: ModSpec.mod_step_io) : SM_Common.input_t :=
-  SM_Common.step_input (fst (ModSpec.step_io_sm spec_io)).
-Definition impl_mem_input (impl_io: ModImpl.mod_step_io) : Log Mem_Common.R_public ContextEnv  :=
-  Mem_Common.step_input (ModImpl.step_io_mem impl_io).
-Definition spec_mem_input (spec_io: ModSpec.mod_step_io) : Mem_Common.input_t :=
-  (Mem_Common.step_input (Mem_Common.ghost_step (ModSpec.step_io_mem spec_io)),
-   (Mem_Common.ghost_input_config0 (ModSpec.step_io_mem spec_io),
-    Mem_Common.ghost_input_config1 (ModSpec.step_io_mem spec_io))).
-Definition impl_core0_feedback (impl_io: ModImpl.mod_step_io) : Core_Common.feedback_t :=
-  Core_Common.step_feedback (ModImpl.step_io_core0 impl_io).
-Definition spec_core0_feedback (spec_io: ModSpec.mod_step_io) : Core_Common.feedback_t :=
-  Core_Common.step_feedback (ModSpec.step_io_core0 spec_io).
-Definition impl_core1_feedback (impl_io: ModImpl.mod_step_io) : Core_Common.feedback_t :=
-  Core_Common.step_feedback (ModImpl.step_io_core1 impl_io).
-Definition spec_core1_feedback (spec_io: ModSpec.mod_step_io) : Core_Common.feedback_t :=
-  Core_Common.step_feedback (ModSpec.step_io_core1 spec_io).
-Definition impl_sm_feedback (impl_io: ModImpl.mod_step_io) : SM_Common.feedback_t :=
-  SM_Common.step_feedback (ModImpl.step_io_sm impl_io).
-Definition spec_sm_feedback (spec_io: ModSpec.mod_step_io) : SM_Common.feedback_t :=
-  SM_Common.step_feedback (fst (ModSpec.step_io_sm spec_io)).
-Definition impl_mem_feedback (impl_io: ModImpl.mod_step_io) : Log Mem_Common.R_public ContextEnv  :=
-  Mem_Common.step_feedback (ModImpl.step_io_mem impl_io).
-Definition spec_mem_feedback (spec_io: ModSpec.mod_step_io) : Mem_Common.feedback_t :=
-  (Mem_Common.step_feedback (Mem_Common.ghost_step (ModSpec.step_io_mem spec_io))).
-
-Ltac fast_destruct_nongoal_matches :=
-  repeat (match goal with
-          | [ H: context[match ?d with | _ => _ end] |- _ ] =>
-              destruct_matches_in d
-              end).
-
-Ltac unfold_spec_props :=
-  consider ModSpec.valid_props;
-  consider ModSpec.valid_P_prop;
-  consider ModSpec.core0_P_prop;
-  consider ModSpec.core1_P_prop;
-  consider ModSpec.sm_P_prop;
-  consider ModSpec.mem_P_prop.
-
-Ltac extract_impl_step__start :=
-  intros; consider ModImpl.do_step_with_metadata; consider ModImpl.compute_mod_outputs;
-    fast_destruct_nongoal_matches; simplify_tupless; simpl in *.
-(* slower QED *)
-Ltac extract_impl_step__step :=
-  consider ModImpl.do_core0; fast_destruct_nongoal_matches; simplify_tupless; simpl in *;
-  consider ModImpl.do_core1; fast_destruct_nongoal_matches; simplify_tupless; simpl in *;
-  consider ModImpl.do_sm; fast_destruct_nongoal_matches; simplify_tupless; simpl in *;
-  consider ModImpl.do_mem; fast_destruct_nongoal_matches; simplify_tupless; simpl in *.
-
-Ltac extract_spec_step__start :=
-  intros; consider ModSpec.do_step_with_metadata; consider ModSpec.compute_mod_outputs;
-    fast_destruct_nongoal_matches; simplify_tupless; simpl in *.
-
-
-Lemma impl_do_step_mem_feedback_empty :
-  forall impl_st impl_st' impl_ev impl_io,
-  ModImpl.do_step_with_metadata impl_st = (impl_st', impl_ev, impl_io) ->
-  impl_mem_feedback impl_io = log_empty.
-Proof.
-  extract_impl_step__start.
-  consider ModImpl.do_mem; fast_destruct_nongoal_matches; simplify_tupless; simpl in *.
-  apply_equiv_eq.
-  consider impl_mem_feedback; simpl.
-  intros; autorewrite with log_helpers; auto.
-Qed.
-
-Lemma spec_do_step_mem_feedback_empty :
-  forall spec_st spec_st' spec_ev spec_io,
-  ModSpec.do_step_with_metadata spec_st = (spec_st', spec_ev, spec_io) ->
-  spec_mem_feedback spec_io = log_empty.
-Proof.
-  extract_spec_step__start.
-  consider ModSpec.do_mem; fast_destruct_nongoal_matches; simplify_tupless; simpl in *.
-  apply_equiv_eq.
-  consider spec_mem_feedback; simpl.
-  intros; autorewrite with log_helpers; auto.
-Qed.
-
-Lemma impl_do_step_core0_input_empty :
-  forall impl_st impl_st' impl_ev impl_io,
-  ModImpl.do_step_with_metadata impl_st = (impl_st', impl_ev, impl_io) ->
-  impl_core0_input impl_io = log_empty.
-Proof.
-  extract_impl_step__start.
-  extract_impl_step__step.
-  consider ModImpl.do_core0; fast_destruct_nongoal_matches; simplify_tupless; simpl in *.
-  consider @Core_Common.proj_log__pub.
-  apply_equiv_eq.
-  consider impl_core0_input.
-  intros; autorewrite with log_helpers; auto.
-Qed.
-
-Lemma spec_do_step_core0_input_empty :
-  forall spec_st spec_st' spec_ev spec_io,
-  ModSpec.do_step_with_metadata spec_st = (spec_st', spec_ev, spec_io) ->
-  spec_core0_input spec_io = log_empty.
-Proof.
-  extract_spec_step__start.
-  consider ModSpec.do_core0; fast_destruct_nongoal_matches; simplify_tupless; simpl in *.
-  consider @Core_Common.proj_log__pub.
-  apply_equiv_eq.
-  intros; autorewrite with log_helpers; auto.
-Qed.
-
-Arguments ModImpl.compute_state : simpl never.
-Lemma impl_core0_do_step_output :
-  forall impl_st impl_st' impl_ev impl_io,
-  ModImpl.do_step_with_metadata impl_st = (impl_st', impl_ev, impl_io) ->
-  fst (core0_do_step_input__koika (ModImpl.state_core0 impl_st)
-                                (impl_core0_input impl_io)) =
-  ModImpl.output_core0 impl_ev.
-Proof.
-  extract_impl_step__start.
-  consider ModImpl.do_core0; fast_destruct_nongoal_matches; simplify_tupless; simpl.
-  unfold_core0_steps.
-  autorewrite with log_helpers in *.
-  consider @Core_Common.do_step_input__koika; simplify_tupless.
-  auto.
-Qed.
-
-Lemma impl_core1_do_step_output :
-  forall impl_st impl_st' impl_ev impl_io,
-  ModImpl.do_step_with_metadata impl_st = (impl_st', impl_ev, impl_io) ->
-  fst (core1_do_step_input__koika (ModImpl.state_core1 impl_st)
-                                (impl_core1_input impl_io)) =
-  ModImpl.output_core1 impl_ev.
-Proof.
-  extract_impl_step__start.
-  consider ModImpl.do_core1; fast_destruct_nongoal_matches; simplify_tupless; simpl.
-  unfold_core1_steps.
-  autorewrite with log_helpers in *.
-  consider @Core_Common.do_step_input__koika; simplify_tupless.
-  auto.
-Qed.
-
-Lemma impl_sm_do_step_output :
-  forall impl_st impl_st' impl_ev impl_io,
-  ModImpl.do_step_with_metadata impl_st = (impl_st', impl_ev, impl_io) ->
-  fst (Impl.System.SM.do_step_input__impl (ModImpl.state_sm impl_st)
-                                        (impl_sm_input impl_io)) =
-  ModImpl.output_sm impl_ev.
-Proof.
-  extract_impl_step__start.
-  consider ModImpl.do_sm; fast_destruct_nongoal_matches; simplify_tupless; simpl.
-  unfold_sm_steps.
-  autorewrite with log_helpers in *.
-  consider @SM_Common.do_step_input__impl; simplify_tupless.
-  auto.
-Qed.
-
-Lemma impl_mem_do_step_output :
-  forall impl_st impl_st' impl_ev impl_io,
-  ModImpl.do_step_with_metadata impl_st = (impl_st', impl_ev, impl_io) ->
-  fst (mem_do_step_input__impl (ModImpl.state_mem impl_st)
-                             (impl_mem_input impl_io)) =
-  ModImpl.output_mem impl_ev.
-Proof.
-  extract_impl_step__start.
-  consider impl_mem_input.
-  consider ModImpl.do_mem; fast_destruct_nongoal_matches; simplify_tupless; simpl.
-  autorewrite with log_helpers in *.
-  rewrite_solve.
-Qed.
-
-Lemma spec_core0_do_step_output :
-  forall spec_st spec_st' spec_ev spec_io,
-  ModSpec.do_step_with_metadata spec_st = (spec_st', spec_ev, spec_io) ->
-  fst (core0_do_step_trans_input__spec (ModSpec.state_core0 spec_st) (spec_core0_input spec_io)) =
-  ModSpec.output_core0 spec_ev.
-Proof.
-  extract_spec_step__start.
-  consider ModSpec.do_core0; fast_destruct_nongoal_matches; simplify_tupless.
-  unfold_core0_steps.
-  autorewrite with log_helpers in *.
-  consider @Core_Common.proj_log__pub.
-  consider @Core_Common.do_step_trans_input__spec; consider @Core_Common.do_step_input__koika; simplify_tupless.
-  simpl.
-  consider spec_core0_input; simpl.
-  auto.
-Qed.
-
-Lemma spec_core1_do_step_output :
-  forall spec_st spec_st' spec_ev spec_io,
-  ModSpec.do_step_with_metadata spec_st = (spec_st', spec_ev, spec_io) ->
-  fst (core1_do_step_trans_input__spec (ModSpec.state_core1 spec_st) (spec_core1_input spec_io)) =
-  ModSpec.output_core1 spec_ev.
-Proof.
-  extract_spec_step__start.
-  consider ModSpec.do_core1; fast_destruct_nongoal_matches; simplify_tupless.
-  unfold_core1_steps.
-  autorewrite with log_helpers in *.
-  consider @Core_Common.proj_log__pub.
-  consider @Core_Common.do_step_trans_input__spec; consider @Core_Common.do_step_input__koika; simplify_tupless.
-  simpl.
-  consider spec_core1_input; simpl.
-  auto.
-Qed.
-
-Lemma spec_sm_do_step_output :
-  forall spec_st spec_st' spec_ev spec_io,
-  ModSpec.do_step_with_metadata spec_st = (spec_st', spec_ev, spec_io) ->
-  Impl.System.SM.do_step_input__spec (ModSpec.state_sm spec_st)
-                                   (spec_sm_input spec_io) =
-  ModSpec.output_sm spec_ev.
-Proof.
-  extract_spec_step__start.
-  consider ModSpec.do_sm; fast_destruct_nongoal_matches; simplify_tupless.
-  unfold_sm_steps.
-  autorewrite with log_helpers in *; simpl.
-  consider spec_sm_input; simpl.
-  auto.
-Qed.
-
-Lemma spec_mem_do_step_output :
-  forall spec_st spec_st' spec_ev spec_io,
-  ModSpec.do_step_with_metadata spec_st = (spec_st', spec_ev, spec_io) ->
-  mem_do_step_trans_input__spec (ModSpec.state_mem spec_st)
-                              (spec_mem_input spec_io) =
-  ModSpec.output_mem spec_ev.
-Proof.
-  extract_spec_step__start.
-  consider ModSpec.do_mem; fast_destruct_nongoal_matches; simplify_tupless.
-  unfold_mem_steps.
-  autorewrite with log_helpers in *; simpl.
-  consider spec_mem_input; simpl.
-  auto.
-Qed.
-
-
-
-Hint Rewrite @SemanticProperties.log_app_empty_l : log_helpers.
-Lemma impl_core1_do_step_input :
-  forall impl_st impl_st' impl_ev impl_io,
-  ModImpl.do_step_with_metadata impl_st = (impl_st', impl_ev, impl_io) ->
-  impl_core1_input impl_io =
-    Core_Common.proj_log__pub
-      (proj_log (REnv' := ContextEnv) Impl.System.Lift_core1 (lift_log Impl.System.Lift_core0 (ModImpl.output_core0 impl_ev))).
-Proof.
-  extract_impl_step__start.
-  consider impl_core1_input; simpl.
-  consider ModImpl.do_core1; fast_destruct_nongoal_matches; simplify_tupless; simpl.
-  consider ModImpl.do_core0; destruct_all_matches; simplify_tupless.
-  autorewrite with log_helpers; auto.
-Qed.
-
-Lemma spec_core1_do_step_input :
-  forall spec_st spec_st' spec_ev spec_io,
-  ModSpec.do_step_with_metadata spec_st = (spec_st', spec_ev, spec_io) ->
-  spec_core1_input spec_io =
-    Core_Common.proj_log__pub
-      (proj_log (REnv' := ContextEnv) Impl.System.Lift_core1 (lift_log Impl.System.Lift_core0 (ModSpec.output_core0 spec_ev))).
-Proof.
-  extract_spec_step__start.
-  consider spec_core1_input; simpl.
-  consider ModSpec.do_core1; fast_destruct_nongoal_matches; simplify_tupless; simpl.
-  consider ModSpec.do_core0; fast_destruct_nongoal_matches; simplify_tupless; simpl.
-  autorewrite with log_helpers.
-  auto.
-Qed.
-
-Lemma impl_sm_do_step_input :
-  forall impl_st impl_st' impl_ev impl_io,
-  ModImpl.do_step_with_metadata impl_st = (impl_st', impl_ev, impl_io) ->
-  impl_sm_input impl_io =
-    SM_Common.proj_log__pub
-      (proj_log (REnv' := ContextEnv) Impl.System.Lift_sm
-                ((lift_log Impl.System.Lift_core1 (ModImpl.output_core1 impl_ev)) ++ (lift_log Impl.System.Lift_core0 (ModImpl.output_core0 impl_ev)))%log).
-Proof.
-  extract_impl_step__start.
-  consider impl_sm_input; simpl.
-  consider ModImpl.do_sm; fast_destruct_nongoal_matches; simplify_tupless; simpl.
-  consider ModImpl.do_core1; fast_destruct_nongoal_matches; simplify_tupless; simpl.
-  consider ModImpl.do_core0; destruct_all_matches; simplify_tupless.
-  autorewrite with log_helpers; auto.
-Qed.
-
-Lemma impl_mem_do_step_input :
-  forall impl_st impl_st' impl_ev impl_io,
-  ModImpl.do_step_with_metadata impl_st = (impl_st', impl_ev, impl_io) ->
-  impl_mem_input impl_io =
-    Mem_Common.proj_log__pub
-      (proj_log (REnv' := ContextEnv) Impl.System.Lift_mem
-                ((lift_log Impl.System.Lift_sm (ModImpl.output_sm impl_ev)) ++
-                 (lift_log Impl.System.Lift_core1 (ModImpl.output_core1 impl_ev)) ++
-                 (lift_log Impl.System.Lift_core0 (ModImpl.output_core0 impl_ev)))%log).
-Proof.
-  extract_impl_step__start.
-  consider impl_mem_input; simpl.
-  consider ModImpl.do_mem; fast_destruct_nongoal_matches; simplify_tupless; simpl.
-  consider ModImpl.do_sm; fast_destruct_nongoal_matches; simplify_tupless; simpl.
-  consider ModImpl.do_core1; fast_destruct_nongoal_matches; simplify_tupless; simpl.
-  consider ModImpl.do_core0; destruct_all_matches; simplify_tupless.
-  autorewrite with log_helpers; auto.
-Qed.
-
-Lemma spec_sm_do_step_input :
-  forall spec_st spec_st' spec_ev spec_io,
-  ModSpec.do_step_with_metadata spec_st = (spec_st', spec_ev, spec_io) ->
-  spec_sm_input spec_io =
-    (SM_Common.proj_log__pub
-      (proj_log (REnv' := ContextEnv) Impl.System.Lift_sm
-                ((lift_log Impl.System.Lift_core1 (ModSpec.output_core1 spec_ev)) ++
-                 (lift_log Impl.System.Lift_core0 (ModSpec.output_core0 spec_ev)))%log)).
-Proof.
-  extract_spec_step__start.
-  consider spec_sm_input; simpl.
-  consider ModSpec.do_sm; fast_destruct_nongoal_matches; simplify_tupless; simpl.
-  consider ModSpec.do_core1; fast_destruct_nongoal_matches; simplify_tupless; simpl.
-  consider ModSpec.do_core0; fast_destruct_nongoal_matches; simplify_tupless; simpl.
-  autorewrite with log_helpers in *.
-  auto.
-Qed.
-
-Lemma spec_mem_do_step_input :
-  forall spec_st spec_st' spec_ev spec_io,
-  ModSpec.do_step_with_metadata spec_st = (spec_st', spec_ev, spec_io) ->
-  spec_mem_input spec_io =
-    (Mem_Common.proj_log__pub
-      (proj_log (REnv' := ContextEnv) Impl.System.Lift_mem
-                ((lift_log Impl.System.Lift_sm (fst (ModSpec.combine_sm_public_output (ModSpec.output_sm spec_ev)))) ++
-                 (lift_log Impl.System.Lift_core1 (ModSpec.output_core1 spec_ev)) ++
-                 (lift_log Impl.System.Lift_core0 (ModSpec.output_core0 spec_ev)))%log),
-      ((ghost_output_config0 (snd (ModSpec.combine_sm_public_output (ModSpec.output_sm spec_ev)))),
-       (ghost_output_config1 (snd (ModSpec.combine_sm_public_output (ModSpec.output_sm spec_ev)))))).
-Proof.
-  extract_spec_step__start.
-  consider spec_mem_input; simpl.
-  consider spec_sm_input; simpl.
-  consider spec_core1_input; simpl.
-  consider spec_core0_input; simpl.
-  consider ModSpec.do_mem; fast_destruct_nongoal_matches; simplify_tupless; simpl.
-  consider ModSpec.do_sm; fast_destruct_nongoal_matches; simplify_tupless; simpl.
-  consider ModSpec.do_core1; fast_destruct_nongoal_matches; simplify_tupless; simpl.
-  consider ModSpec.do_core0; fast_destruct_nongoal_matches; simplify_tupless; simpl.
-  rewrite Heqp0; simpl.
-  autorewrite with log_helpers in *.
-  auto.
-Qed.
-
-Lemma cores_do_not_share_registers :
-  ~ (exists reg1 reg2, rlift Impl.System.Lift_core0 reg1 = rlift Impl.System.Lift_core1 reg2).
-Proof.
-  intuition.
-  destruct reg1; destruct reg2; simpl in *;
-    consider Impl.System.Lift_core0; consider Impl.System.Lift_core1;
-    consider Impl.System.core0_public_lift; consider Impl.System.core1_public_lift;
-      destruct_all_matches; congruence.
-Qed.
-
-
-
-
-Lemma proj_core1_lift_core0_log_equiv :
-  forall log1 log2,
-  Core_Common.proj_log__pub log1 = Core_Common.proj_log__pub log2 ->
-  proj_log (REnv := ContextEnv) (REnv' := ContextEnv) Impl.System.Lift_core1 (lift_log Impl.System.Lift_core0 log1) =
-  proj_log (REnv' := ContextEnv) Impl.System.Lift_core1 (lift_log Impl.System.Lift_core0 log2).
-Proof.
-  intros.
-  consider @Core_Common.proj_log__pub.
-  consider @proj_log.
-  apply_equiv_eq.
-  intros.
-  repeat rewrite getenv_create.
-  destruct k.
-  - repeat rewrite getenv_lift_log_not_exists; auto;
-      intuition; apply cores_do_not_share_registers;
-      eexists; eexists; eauto.
-  - repeat rewrite getenv_lift_log_not_exists; auto;
-      intuition; apply cores_do_not_share_registers;
-      eexists; eexists; eauto.
-Qed.
-
-Lemma valid_props_extract_core1_valid_input :
-  forall ios spec_st0 t initial_dram n,
-  ModSpec.step_n_with_metadata initial_dram n = (spec_st0, t, ios) ->
-  ModSpec.valid_props initial_dram (ios ++ [snd (ModSpec.do_step_with_metadata spec_st0)]) ->
-  core1_valid_input (ModSpec.state_core1 spec_st0) (spec_core1_input (snd (ModSpec.do_step_with_metadata spec_st0))).
-Admitted.
-
-Lemma valid_props_extract_sm_valid_input :
-  forall ios spec_st0 t initial_dram n,
-  ModSpec.step_n_with_metadata initial_dram n = (spec_st0, t, ios) ->
-  ModSpec.valid_props initial_dram (ios ++ [snd (ModSpec.do_step_with_metadata spec_st0)]) ->
-  sm_valid_input (ModSpec.state_sm spec_st0) (spec_sm_input (snd (ModSpec.do_step_with_metadata spec_st0))).
-Admitted.
-
-Lemma valid_props_extract_mem_valid_input :
-  forall ios spec_st0 t initial_dram n,
-  ModSpec.step_n_with_metadata initial_dram n = (spec_st0, t, ios) ->
-  ModSpec.valid_props initial_dram (ios ++ [snd (ModSpec.do_step_with_metadata spec_st0)]) ->
-  mem_valid_input (ModSpec.state_mem spec_st0) (spec_mem_input (snd (ModSpec.do_step_with_metadata spec_st0))).
-Admitted.
-
-
-
-Axiom __magic__ : forall T, T.
-Tactic Notation "__magic" := apply __magic__.
-
-Lemma proj_sm_lift_core0_log_equiv :
-  forall log1 log1' ,
-  Core_Common.proj_log__pub log1 = Core_Common.proj_log__pub log1' ->
-    (proj_log (REnv := ContextEnv) (REnv' := ContextEnv) Impl.System.Lift_sm
-       (lift_log Impl.System.Lift_core0 log1)) =
-    (proj_log (REnv' := ContextEnv) Impl.System.Lift_sm
-       (lift_log Impl.System.Lift_core0 log1')).
-Proof.
-  intros. consider @Core_Common.proj_log__pub.
-  consider @proj_log.
-  apply_equiv_eq; intros; repeat rewrite getenv_create.
-  destruct k.
-  - admit.
-  - repeat rewrite getenv_lift_log_not_exists; auto; intuition;
-      simpl in *; destruct reg; simpl in *; try congruence;
-      destruct r; simpl in *; congruence.
-Admitted.
-
-Lemma proj_sm_lift_core1_log_equiv :
-  forall log1 log1' ,
-  Core_Common.proj_log__pub log1 = Core_Common.proj_log__pub log1' ->
-    (proj_log (REnv := ContextEnv) (REnv' := ContextEnv) Impl.System.Lift_sm
-       (lift_log Impl.System.Lift_core1 log1)) =
-    (proj_log (REnv' := ContextEnv) Impl.System.Lift_sm
-       (lift_log Impl.System.Lift_core1 log1')).
-Admitted.
-
-Lemma proj_mem_lift_core1_log_equiv :
-  forall log1 log1' ,
-  Core_Common.proj_log__pub log1 = Core_Common.proj_log__pub log1' ->
-    (proj_log (REnv := ContextEnv) (REnv' := ContextEnv) Impl.System.Lift_mem
-       (lift_log Impl.System.Lift_core1 log1)) =
-    (proj_log (REnv' := ContextEnv) Impl.System.Lift_mem
-       (lift_log Impl.System.Lift_core1 log1')).
-Admitted.
-
-Lemma proj_mem_lift_core0_log_equiv :
-  forall log1 log1' ,
-  Core_Common.proj_log__pub log1 = Core_Common.proj_log__pub log1' ->
-    (proj_log (REnv := ContextEnv) (REnv' := ContextEnv) Impl.System.Lift_mem
-       (lift_log Impl.System.Lift_core0 log1)) =
-    (proj_log (REnv' := ContextEnv) Impl.System.Lift_mem
-       (lift_log Impl.System.Lift_core0 log1')).
-Admitted.
-
-Lemma proj_mem_lift_sm_log_equiv :
-  forall log1 log1' ,
-  SM_Common.proj_log__pub log1 = SM_Common.proj_log__pub log1' ->
-    (proj_log (REnv := ContextEnv) (REnv' := ContextEnv) Impl.System.Lift_mem
-       (lift_log Impl.System.Lift_sm log1)) =
-    (proj_log (REnv' := ContextEnv) Impl.System.Lift_mem
-       (lift_log Impl.System.Lift_sm log1')).
-Admitted.
-
-Ltac solve_lift_log_not_exists :=
-  repeat match goal with
-  | |- not (exists reg, rlift _ reg = _)  =>
-      clear; intuition; simpl in *; destruct reg; simpl in *; try congruence
-  | H: Impl.System.mem_public_lift ?r = _ |- _ =>
-      destruct r; simpl in *; try congruence
-  end.
-
-Lemma mem_output_log_equiv_impl_combine_public_output :
-  forall impl_out spec_out,
-  mem_output_log_equivalent impl_out spec_out ->
-  (proj_log (REnv := ContextEnv) (REnv' := ContextEnv) Impl.System.Lift_sm (lift_log Impl.System.Lift_mem impl_out)) =
-  (proj_log (REnv' := ContextEnv) Impl.System.Lift_sm
-       (lift_log Impl.System.Lift_mem (ModSpec.combine_mem_public_output spec_out))).
-Proof.
-  intros. consider mem_output_log_equivalent.
-  apply_equiv_eq.
-  intros; repeat rewrite getenv_create.
-  consider ModSpec.combine_mem_public_output; simpl.
-  destruct spec_out; simpl.
-  consider @Mem_Common.output_log_equivalent.
-  unfold proj_log. repeat rewrite getenv_create.
-  simpl_eqs.
-  destruct k; simpl.
-  - admit. (* lift annoying *)
-  - repeat rewrite getenv_lift_log_not_exists; auto;
-      solve_lift_log_not_exists.
-Admitted.
-
-Lemma proj_core1_lift_mem_equiv :
-  forall log1 log2,
-  mem_output_log_equivalent log1 log2 ->
-  proj_log (REnv := ContextEnv) (REnv' := ContextEnv) Impl.System.Lift_core1 (lift_log Impl.System.Lift_mem log1) =
-  proj_log (REnv' := ContextEnv) Impl.System.Lift_core1 (lift_log Impl.System.Lift_mem (ModSpec.combine_mem_public_output log2)).
-Admitted.
-
-Lemma proj_core0_lift_mem_equiv :
-  forall log1 log2,
-  mem_output_log_equivalent log1 log2 ->
-  proj_log (REnv := ContextEnv) (REnv' := ContextEnv) Impl.System.Lift_core0 (lift_log Impl.System.Lift_mem log1) =
-  proj_log (REnv' := ContextEnv) Impl.System.Lift_core0 (lift_log Impl.System.Lift_mem (ModSpec.combine_mem_public_output log2)).
-Admitted.
-
-Lemma proj_core0_lift_sm_equiv :
-  forall log1 log2,
-  sm_output_log_equivalent log1 log2 ->
-  proj_log (REnv := ContextEnv) (REnv' := ContextEnv) Impl.System.Lift_core0 (lift_log Impl.System.Lift_sm log1) =
-  proj_log (REnv' := ContextEnv) Impl.System.Lift_core0 (lift_log Impl.System.Lift_sm (fst (ModSpec.combine_sm_public_output log2))).
-Admitted.
-
-Lemma proj_core0_lift_core1_equiv :
-  forall log1 log2,
-  core1_output_log_equivalent log1 log2 ->
-  proj_log (REnv := ContextEnv) (REnv' := ContextEnv) Impl.System.Lift_core0 (lift_log Impl.System.Lift_core1 log1) =
-  proj_log (REnv' := ContextEnv) Impl.System.Lift_core0 (lift_log Impl.System.Lift_core1 log2).
-Admitted.
-
-
-Lemma proj_core1_lift_sm_equiv :
-  forall log1 log2,
-  sm_output_log_equivalent log1 log2 ->
-  proj_log (REnv := ContextEnv) (REnv' := ContextEnv) Impl.System.Lift_core1 (lift_log Impl.System.Lift_sm log1) =
-  proj_log (REnv' := ContextEnv) Impl.System.Lift_core1 (lift_log Impl.System.Lift_sm (fst (ModSpec.combine_sm_public_output log2))).
-Admitted.
-
-
-
-Lemma sm_output_log_equiv_impl_combine_public_output :
-  forall impl_out spec_out,
-  SM_Common.output_log_equivalent impl_out spec_out ->
-  SM_Common.proj_log__pub impl_out =
-  SM_Common.proj_log__pub (fst (ModSpec.combine_sm_public_output spec_out)).
-Proof.
-  intros. consider SM_Common.output_log_equivalent.
-  apply_equiv_eq.
-  intros. consider SM_Common.proj_log__pub.
-  repeat rewrite getenv_create.
-  consider ModSpec.combine_sm_public_output; simpl.
-  destruct spec_out; simpl. rewrite getenv_create.
-  specialize H with (reg := SM_Common.public k).
-  simpl in H.
-  destruct_all_matches; auto.
-Qed.
-
-Lemma impl_sm_do_step_feedback :
-  forall impl_st impl_st' impl_ev impl_io,
-  ModImpl.do_step_with_metadata impl_st = (impl_st', impl_ev, impl_io) ->
-  SM_Common.step_feedback (ModImpl.step_io_sm impl_io) =
-  SM_Common.proj_log__pub
-    (proj_log (REnv' := ContextEnv) Impl.System.Lift_sm
-              (lift_log Impl.System.Lift_mem (ModImpl.output_mem impl_ev))).
-Proof.
-  extract_impl_step__start.
-  consider ModImpl.do_sm; fast_destruct_nongoal_matches; simplify_tupless; simpl.
-  consider ModImpl.do_mem; fast_destruct_nongoal_matches; simplify_tupless; simpl.
-  rewrite SemanticProperties.log_app_empty_r; auto.
-Qed.
-Lemma spec_sm_do_step_feedback :
-  forall spec_st spec_st' spec_ev spec_io,
-  ModSpec.do_step_with_metadata spec_st = (spec_st', spec_ev, spec_io) ->
-  SM_Common.step_feedback (fst (ModSpec.step_io_sm spec_io)) =
-  SM_Common.proj_log__pub
-    (proj_log (REnv' := ContextEnv) Impl.System.Lift_sm
-              (lift_log Impl.System.Lift_mem (ModSpec.combine_mem_public_output (ModSpec.output_mem spec_ev)))).
-Proof.
-  extract_spec_step__start.
-  rewrite SemanticProperties.log_app_empty_r; auto.
-  consider ModSpec.do_mem; fast_destruct_nongoal_matches; simplify_tupless; simpl.
-  consider ModSpec.do_sm; fast_destruct_nongoal_matches; simplify_tupless; simpl.
-  auto.
-Qed.
-Lemma impl_core1_do_step_feedback :
-  forall impl_st impl_st' impl_ev impl_io,
-  ModImpl.do_step_with_metadata impl_st = (impl_st', impl_ev, impl_io) ->
-  Core_Common.step_feedback (ModImpl.step_io_core1 impl_io) =
-  Core_Common.proj_log__pub
-    (proj_log (REnv' := ContextEnv) Impl.System.Lift_core1
-              ((lift_log Impl.System.Lift_mem (ModImpl.output_mem impl_ev))++
-               (lift_log Impl.System.Lift_sm (ModImpl.output_sm impl_ev)))%log).
-Proof.
-  extract_impl_step__start.
-  consider ModImpl.do_core1; fast_destruct_nongoal_matches; simplify_tupless; simpl.
-  consider ModImpl.do_sm; fast_destruct_nongoal_matches; simplify_tupless; simpl.
-  consider ModImpl.do_mem; fast_destruct_nongoal_matches; simplify_tupless; simpl.
-  rewrite SemanticProperties.log_app_empty_r; auto.
-Qed.
-Lemma spec_core1_do_step_feedback :
-  forall spec_st spec_st' spec_ev spec_io,
-  ModSpec.do_step_with_metadata spec_st = (spec_st', spec_ev, spec_io) ->
-  Core_Common.step_feedback (ModSpec.step_io_core1 spec_io) =
-  Core_Common.proj_log__pub
-    (proj_log (REnv' := ContextEnv) Impl.System.Lift_core1
-              ((lift_log Impl.System.Lift_mem (ModSpec.combine_mem_public_output ((ModSpec.output_mem spec_ev))))++
-               (lift_log Impl.System.Lift_sm (fst (ModSpec.combine_sm_public_output (ModSpec.output_sm spec_ev))))%log)%log).
-Proof.
-  extract_spec_step__start.
-  rewrite SemanticProperties.log_app_empty_r; auto.
-  consider ModSpec.do_mem; fast_destruct_nongoal_matches; simplify_tupless; simpl.
-  consider ModSpec.do_sm; fast_destruct_nongoal_matches; simplify_tupless; simpl.
-  consider ModSpec.do_core1; fast_destruct_nongoal_matches; simplify_tupless; simpl.
-  rewrite Heqp0; simpl.
-  rewrite SemanticProperties.log_app_assoc; auto.
-Qed.
-
-Lemma impl_core0_do_step_feedback :
-  forall impl_st impl_st' impl_ev impl_io,
-  ModImpl.do_step_with_metadata impl_st = (impl_st', impl_ev, impl_io) ->
-  Core_Common.step_feedback (ModImpl.step_io_core0 impl_io) =
-  Core_Common.proj_log__pub
-    (proj_log (REnv' := ContextEnv) Impl.System.Lift_core0
-              ((lift_log Impl.System.Lift_mem (ModImpl.output_mem impl_ev))++
-               (lift_log Impl.System.Lift_sm (ModImpl.output_sm impl_ev))++
-               (lift_log Impl.System.Lift_core1 (ModImpl.output_core1 impl_ev)))%log).
-Proof.
-  extract_impl_step__start.
-  consider ModImpl.do_core0; fast_destruct_nongoal_matches; simplify_tupless; simpl.
-  consider ModImpl.do_core1; fast_destruct_nongoal_matches; simplify_tupless; simpl.
-  consider ModImpl.do_sm; fast_destruct_nongoal_matches; simplify_tupless; simpl.
-  consider ModImpl.do_mem; fast_destruct_nongoal_matches; simplify_tupless; simpl.
-  rewrite SemanticProperties.log_app_empty_r.
-  rewrite SemanticProperties.log_app_assoc; auto.
-Qed.
-
-Lemma spec_core0_do_step_feedback :
-  forall spec_st spec_st' spec_ev spec_io,
-  ModSpec.do_step_with_metadata spec_st = (spec_st', spec_ev, spec_io) ->
-  Core_Common.step_feedback (ModSpec.step_io_core0 spec_io) =
-  Core_Common.proj_log__pub
-    (proj_log (REnv' := ContextEnv) Impl.System.Lift_core0
-              ((lift_log Impl.System.Lift_mem (ModSpec.combine_mem_public_output ((ModSpec.output_mem spec_ev))))++
-               (lift_log Impl.System.Lift_sm (fst (ModSpec.combine_sm_public_output (ModSpec.output_sm spec_ev))))++
-               (lift_log Impl.System.Lift_core1 (ModSpec.output_core1 spec_ev))
-               )%log).
-Proof.
-  extract_spec_step__start.
-  rewrite SemanticProperties.log_app_empty_r; auto.
-  consider ModSpec.do_mem; fast_destruct_nongoal_matches; simplify_tupless; simpl.
-  consider ModSpec.do_sm; fast_destruct_nongoal_matches; simplify_tupless; simpl.
-  consider ModSpec.do_core1; fast_destruct_nongoal_matches; simplify_tupless; simpl.
-  consider ModSpec.do_core0; fast_destruct_nongoal_matches; simplify_tupless; simpl.
-  rewrite SemanticProperties.log_app_assoc; auto.
-  rewrite Heqp0; simpl.
-  repeat rewrite SemanticProperties.log_app_assoc; auto.
-Qed.
-
           (* ======== Equiv inputs/outputs, forward ========= *)
-          assert (impl_core0_input impl_io = log_empty) as HImplCore0Empty
-             by (eapply impl_do_step_core0_input_empty; eauto).
-          assert (spec_core0_input spec_io = log_empty) as HSpecCore0Empty
-             by (eapply spec_do_step_core0_input_empty; eauto).
+          assert (ModImpl.core0_input impl_io = log_empty) as HImplCore0Empty
+             by (eapply ModImpl.do_step_core0_input_empty; eauto).
+          assert (ModSpec.core0_input spec_io = log_empty) as HSpecCore0Empty
+             by (eapply ModSpec.do_step_core0_input_empty; eauto).
           (* Core0 input eq *)
-          assert (impl_core0_input impl_io = spec_core0_input spec_io) as Heq_core0_input.
+          assert (ModImpl.core0_input impl_io = ModSpec.core0_input spec_io) as Heq_core0_input.
           { rewrite_solve. }
           (* Core0 output eq *)
           assert (core0_output_log_equivalent (ModImpl.output_core0 impl_ev)
                                               (ModSpec.output_core0 spec_ev)) as Heq_core0_output.
           { rewrite forall_sim_step_extract_core0 with (1 := IHn) in *.
             consider core0_output_log_equivalent.
-            eapply Core0.output_correctness with (input := impl_core0_input impl_io); eauto.
+            eapply Core0.output_correctness with (input := ModImpl.core0_input impl_io); eauto.
             - rewrite_term_from_tuple prop_core0; unfold_spec_props; intuition.
             - rewrite_term_from_tuple prop_core0; unfold_spec_props; intuition.
-            - rewrite<-impl_core0_do_step_output with (1 := HImplStep); auto.
-            - rewrite<-spec_core0_do_step_output with (1 := HSpecStep); unfold_core0_steps; rewrite_solve.
+            - rewrite<-ModImpl.core0_do_step_output with (1 := HImplStep); auto.
+            - rewrite<-ModSpec.core0_do_step_output with (1 := HSpecStep); unfold_core0_steps; rewrite_solve.
           }
           (* Core1 input *)
-          assert (impl_core1_input impl_io = spec_core1_input spec_io) as Heq_core1_input.
+          assert (ModImpl.core1_input impl_io = ModSpec.core1_input spec_io) as Heq_core1_input.
           {
-            rewrite impl_core1_do_step_input with (1 := HImplStep).
-            rewrite spec_core1_do_step_input with (1 := HSpecStep).
+            rewrite ModImpl.core1_do_step_input with (1 := HImplStep).
+            rewrite ModSpec.core1_do_step_input with (1 := HSpecStep).
             consider core0_output_log_equivalent.
             consider @Core_Common.output_log_equivalent.
             consider @Core_Common.ext_log_equivalent.
@@ -2297,19 +2297,19 @@ Qed.
                                               (ModSpec.output_core1 spec_ev)) as Heq_core1_output.
           { rewrite forall_sim_step_extract_core1 with (1 := IHn) in *.
             consider core1_output_log_equivalent.
-            eapply Core1.output_correctness with (input := spec_core1_input spec_io); eauto.
+            eapply Core1.output_correctness with (input := ModSpec.core1_input spec_io); eauto.
             - rewrite_term_from_tuple prop_core1; clear - HSpecProp; unfold_spec_props; propositional.
             - rewrite_term_from_tuple prop_core1; clear - HSpecProp; unfold_spec_props; propositional.
             - rewrite_term_from_tuple spec_io.
-              eapply valid_props_extract_core1_valid_input; eauto.
+              eapply ModSpec.valid_props_extract_core1_valid_input; eauto.
               rewrite_solve.
-            - rewrite<-impl_core1_do_step_output with (1 := HImplStep); rewrite_solve.
-            - rewrite<-spec_core1_do_step_output with (1 := HSpecStep); auto.
+            - rewrite<-ModImpl.core1_do_step_output with (1 := HImplStep); rewrite_solve.
+            - rewrite<-ModSpec.core1_do_step_output with (1 := HSpecStep); auto.
           }
           (* SM input *)
-          assert (impl_sm_input impl_io = spec_sm_input spec_io) as Heq_sm_input.
-          { rewrite impl_sm_do_step_input with (1 := HImplStep).
-            rewrite spec_sm_do_step_input with (1 := HSpecStep).
+          assert (ModImpl.sm_input impl_io = ModSpec.sm_input spec_io) as Heq_sm_input.
+          { rewrite ModImpl.sm_do_step_input with (1 := HImplStep).
+            rewrite ModSpec.sm_do_step_input with (1 := HSpecStep).
             consider core0_output_log_equivalent.
             consider core1_output_log_equivalent.
             consider SM_Common.proj_log__pub.
@@ -2320,26 +2320,24 @@ Qed.
             erewrite proj_sm_lift_core1_log_equiv; eauto.
           }
           (* SM output *)
-          assert (sm_output_log_equivalent (ModImpl.output_sm impl_ev)
-                                            (ModSpec.output_sm spec_ev)) as Heq_sm_output.
+          assert (SM_Common.output_log_equivalent (ModImpl.output_sm impl_ev)
+                                                  (ModSpec.output_sm spec_ev)) as Heq_sm_output.
           { rewrite forall_sim_step_extract_sm with (1 := IHn) in *.
-            consider sm_output_log_equivalent.
             consider Impl.System.SM.do_steps__spec.
             consider Impl.System.SM.do_steps__impl.
-            apply SM_Common.output_correctness with (input := spec_sm_input spec_io) (3 := HSpecSM) (4 := HImplSM).
+            apply SM_Common.output_correctness with (input := ModSpec.sm_input spec_io) (3 := HSpecSM) (4 := HImplSM).
             - rewrite_term_from_tuple prop_sm; clear - HSpecProp; unfold_spec_props; propositional.
             - rewrite_term_from_tuple prop_sm; clear - HSpecProp; unfold_spec_props; propositional.
             - rewrite_term_from_tuple spec_io.
-              eapply valid_props_extract_sm_valid_input; eauto.
+              eapply ModSpec.valid_props_extract_sm_valid_input; eauto.
               rewrite_solve.
-            - rewrite<-impl_sm_do_step_output with (1 := HImplStep); rewrite_solve.
-            - rewrite<-spec_sm_do_step_output with (1 := HSpecStep); auto.
+            - rewrite<-ModImpl.sm_do_step_output with (1 := HImplStep); rewrite_solve.
+            - rewrite<-ModSpec.sm_do_step_output with (1 := HSpecStep); auto.
           }
           (* Mem input *)
-          assert (impl_mem_input impl_io = fst (spec_mem_input spec_io)) as Heq_mem_input.
-          { rewrite impl_mem_do_step_input with (1 := HImplStep).
-            rewrite spec_mem_do_step_input with (1 := HSpecStep).
-            consider sm_output_log_equivalent.
+          assert (ModImpl.mem_input impl_io = fst (ModSpec.mem_input spec_io)) as Heq_mem_input.
+          { rewrite ModImpl.mem_do_step_input with (1 := HImplStep).
+            rewrite ModSpec.mem_do_step_input with (1 := HSpecStep).
             consider core0_output_log_equivalent.
             consider core1_output_log_equivalent.
             consider @Mem_Common.proj_log__pub.
@@ -2360,23 +2358,23 @@ Qed.
             consider mem_do_steps__impl.
             consider mem_do_steps__spec.
             pose proof Memory.output_correctness as MemOutputCorrect. consider @Mem_Common.P_output_correctness.
-            eapply MemOutputCorrect with (input := spec_mem_input spec_io); eauto.
+            eapply MemOutputCorrect with (input := ModSpec.mem_input spec_io); eauto.
             - rewrite_term_from_tuple prop_mem; clear - HSpecProp; unfold_spec_props; propositional.
             - rewrite_term_from_tuple prop_mem; clear - HSpecProp; unfold_spec_props; propositional.
             - rewrite_term_from_tuple spec_io.
-              eapply valid_props_extract_mem_valid_input; eauto.
+              eapply ModSpec.valid_props_extract_mem_valid_input; eauto.
               rewrite_solve.
-            - rewrite<-impl_mem_do_step_output with (1 := HImplStep); rewrite_solve.
-            - rewrite<-spec_mem_do_step_output with (1 := HSpecStep); auto.
+            - rewrite<-ModImpl.mem_do_step_output with (1 := HImplStep); rewrite_solve.
+            - rewrite<-ModSpec.mem_do_step_output with (1 := HSpecStep); auto.
           }
 
           (* ======= Equiv feedback, backwards ====== *)
           assert (Mem_Common.step_feedback (ModImpl.step_io_mem impl_io) = log_empty) as HImplMemFBEmpty.
-          { eapply impl_do_step_mem_feedback_empty; eauto.
+          { eapply ModImpl.do_step_mem_feedback_empty; eauto.
           }
           assert (Mem_Common.step_feedback (Mem_Common.ghost_step (ModSpec.step_io_mem spec_io)) = log_empty)
             as HSpecMemFBEmpty.
-          { eapply spec_do_step_mem_feedback_empty; eauto. }
+          { eapply ModSpec.do_step_mem_feedback_empty; eauto. }
           assert (Mem_Common.step_feedback (ModImpl.step_io_mem impl_io)
                   = Mem_Common.step_feedback (Mem_Common.ghost_step (ModSpec.step_io_mem spec_io)))
             as Heq_mem_feedback
@@ -2384,16 +2382,16 @@ Qed.
           assert (SM_Common.step_feedback (ModImpl.step_io_sm impl_io)
                   = SM_Common.step_feedback (fst (ModSpec.step_io_sm spec_io)))
             as Heq_sm_feedback.
-          { rewrite impl_sm_do_step_feedback with (1 := HImplStep).
-            rewrite spec_sm_do_step_feedback with (1 := HSpecStep).
+          { rewrite ModImpl.sm_do_step_feedback with (1 := HImplStep).
+            rewrite ModSpec.sm_do_step_feedback with (1 := HSpecStep).
             apply f_equal.
             apply mem_output_log_equiv_impl_combine_public_output; auto.
           }
           assert (Core_Common.step_feedback (ModImpl.step_io_core1 impl_io)
                   = Core_Common.step_feedback (ModSpec.step_io_core1 spec_io))
             as Heq_core1_feedback.
-          { rewrite impl_core1_do_step_feedback with (1 := HImplStep).
-            rewrite spec_core1_do_step_feedback with (1 := HSpecStep).
+          { rewrite ModImpl.core1_do_step_feedback with (1 := HImplStep).
+            rewrite ModSpec.core1_do_step_feedback with (1 := HSpecStep).
             apply f_equal.
             repeat rewrite<-log_app_comm_proj_log.
             erewrite proj_core1_lift_mem_equiv; eauto.
@@ -2402,28 +2400,14 @@ Qed.
           assert (Core_Common.step_feedback (ModImpl.step_io_core0 impl_io)
                   = Core_Common.step_feedback (ModSpec.step_io_core0 spec_io))
             as Heq_core0_feedback.
-          { rewrite impl_core0_do_step_feedback with (1 := HImplStep).
-            rewrite spec_core0_do_step_feedback with (1 := HSpecStep).
+          { rewrite ModImpl.core0_do_step_feedback with (1 := HImplStep).
+            rewrite ModSpec.core0_do_step_feedback with (1 := HSpecStep).
             apply f_equal.
             repeat rewrite<-log_app_comm_proj_log.
             erewrite proj_core0_lift_mem_equiv; eauto.
             erewrite proj_core0_lift_sm_equiv; eauto.
             erewrite proj_core0_lift_core1_equiv; eauto.
           }
-
-
-
-
-Ltac unfold_short_ios :=
-  consider impl_core0_input;
-  consider impl_core1_input;
-  consider impl_sm_input;
-  consider impl_mem_input;
-  consider spec_core0_input;
-  consider spec_core1_input;
-  consider spec_sm_input;
-  consider spec_mem_input.
-
           (* ======= Solve ====== *)
           constructor;
             destruct_with_eqn impl_io; destruct_with_eqn spec_io; simpl in *;
